Try to implement automatic lookup of assumptions in "theorem assumes ... shows ..." statements, instead of having to explicitly declare typings

HoTT_Base.thy
@@ -13,7 +13,9 @@ Among other things, it:
 
 theory HoTT_Base
 imports Pure
-keywords "assume_type" "assume_types" :: thy_decl
+keywords
+  "theorem*" "lemma*" "corollary*" "proposition*" :: thy_goal and
+  "schematic_goal*" :: thy_goal
 
 begin
 
@@ -34,29 +36,44 @@ text \<open>Set up type assumption and inference functionality:\<close>
 
 ML_file "util.ML"
 ML_file "typing.ML"
-ML \<open>
-val _ =
-  let
-    fun store_typing ctxt = Typing.put_declared_typing o (Syntax.read_prop ctxt)
-  in
-    Outer_Syntax.local_theory
-      @{command_keyword "assume_type"}
-      "Declare typing assumptions"
-      (Parse.prop >>
-        (fn prop => fn lthy => Local_Theory.background_theory (store_typing lthy prop) lthy))
-  end
 
-val _ =
-  let
-    val parser = Parse.and_list (Parse.prop)
-    fun store_typings ctxt = fold (Typing.put_declared_typing o (Syntax.read_prop ctxt))
-  in
-    Outer_Syntax.local_theory
-      @{command_keyword "assume_types"}
-      "Declare typing assumptions"
-      (parser >>
-        (fn props => fn lthy => Local_Theory.background_theory (store_typings lthy props) lthy))
-  end
+text \<open>
+Set up keywords @{theory_text "theorem*"}, @{theory_text "lemma*"} etc.—theorem environments with type inference.
+\<close>
+
+ML \<open>
+(* This code is copied and modified from the original in src/Pure/Pure.thy *)
+let
+val long_keyword =
+  Parse_Spec.includes >> K "" ||
+  Parse_Spec.long_statement_keyword;
+
+val long_statement =
+  Scan.optional (Parse_Spec.opt_thm_name ":" --| Scan.ahead long_keyword) Binding.empty_atts --
+  Scan.optional Parse_Spec.includes [] -- Parse_Spec.long_statement
+    >> (fn ((binding, includes), (elems, concl)) => (true, binding, includes, elems, concl));
+
+val short_statement =
+  Parse_Spec.statement -- Parse_Spec.if_statement -- Parse.for_fixes
+    >> (fn ((shows, assumes), fixes) =>
+      (false, Binding.empty_atts, [], [Element.Fixes fixes, Element.Assumes assumes],
+        Element.Shows shows));
+
+fun theorem cmd schematic descr =
+  Outer_Syntax.local_theory_to_proof' cmd ("State " ^ descr ^ " with type inference")
+    ((long_statement || short_statement) >>
+      (fn (long, binding, includes, elems, concl) =>
+        (if schematic then Specification.schematic_theorem_cmd else Specification.theorem_cmd)
+          long Thm.theoremK NONE (K I) binding includes elems concl))
+in
+(
+theorem @{command_keyword "theorem*"} false "theorem";
+theorem @{command_keyword "lemma*"} false "lemma";
+theorem @{command_keyword "corollary*"} false "corollary";
+theorem @{command_keyword "proposition*"} false "proposition";
+theorem @{command_keyword "schematic_goal*"} true "schematic goal"
+)
+end
 \<close>
                                                                                   
 section \<open>Universes\<close>
